RiscvDialect/Instructions/llvm_instructions.lean
@@ -1,5 +1,3 @@
-import RiscvDialect.RDialect
-import RiscvDialect.RefinementDialect
 import SSA.Projects.InstCombine.LLVM.Semantics
 import SSA.Projects.InstCombine.LLVM.PrettyEDSL
 import SSA.Projects.InstCombine.Refinement
@@ -9,7 +7,7 @@ import SSA.Projects.InstCombine.Base
 import SSA.Projects.InstCombine.ForLean
 import Lean
 
-/-- this file contains a collection of llvm programs that each modell one instruction. 
+/-- this file contains a collection of llvm programs that each modell one instruction.
 
 -/
 
