RiscvDialect/RISCV64/RISCVExamples.lean
@@ -1,5 +1,7 @@
 
-import RiscvDialect.Dialect
+import RiscvDialect.RISCV64.Syntax
+import RiscvDialect.RISCV64.Base
+import RiscvDialect.RISCV64.Semantics
 import SSA.Core.Tactic
 import SSA.Core.ErasedContext
 import SSA.Core.HVector
@@ -7,7 +9,7 @@ import SSA.Core.EffectKind
 import SSA.Core.Util
 
 open MLIR AST in
-
+open RISCV64
 /-- contains riscv dialect and evaultes them. Purpose was to check the semantics of my dialect and to get familar with
  invkoing it on an IR level. -/
 
@@ -34,10 +36,10 @@ def RISCVEg2 := [RV64_com| {
 
 
 #check HVector.cons (BitVec.ofNat 64 1) .nil
-#check HVector TyDenote.toType [toRISCV.Ty.bv]
+#check HVector TyDenote.toType [RISCV64.Ty.bv]
 #check HVector -- returns a function from List α to lub type universe of both types.
 
-def lh : HVector TyDenote.toType [toRISCV.Ty.bv] :=  HVector.cons (BitVec.ofNat 64 1) .nil
+def lh : HVector TyDenote.toType [RISCV64.Ty.bv] :=  HVector.cons (BitVec.ofNat 64 1) .nil
 def test_selfadd : BitVec 64 := RISCVEg2.denote (Ctxt.Valuation.ofHVector lh)
 #eval test_selfadd
 
@@ -48,7 +50,7 @@ def RISCVEg3 := [RV64_com| {
     "return" (%2) : (!i64, !i64 ) -> ()
 }]
 --def lh3 : HVector TyDenote.toType [toRISCV.Ty.bv ,toRISCV.Ty.bv] :=  HVector.cons (BitVec.ofNat 64 1) <| HVector.cons (BitVec.ofNat 64 2) .nil
-def lh3 : HVector TyDenote.toType [toRISCV.Ty.bv ,toRISCV.Ty.bv] :=  HVector.cons (BitVec.ofNat 64 0) <| HVector.cons (BitVec.ofNat 64 2) .nil --checking edge cases
+def lh3 : HVector TyDenote.toType [RISCV64.Ty.bv ,RISCV64.Ty.bv] :=  HVector.cons (BitVec.ofNat 64 0) <| HVector.cons (BitVec.ofNat 64 2) .nil --checking edge cases
 def test_addw : BitVec 64 := RISCVEg3.denote  (Ctxt.Valuation.ofHVector lh3)
 #eval test_addw
 
@@ -60,7 +62,7 @@ def RISCVEg4 := [RV64_com| {
     %2 = "RV64.sllw" (%0, %1) : (!i64, !i64) -> (!i64)
     "return" (%2) : (!i64, !i64 ) -> ()
 }]
-def lh4 : HVector TyDenote.toType [toRISCV.Ty.bv ,toRISCV.Ty.bv] :=  HVector.cons (BitVec.ofNat 64 2) <| HVector.cons (BitVec.ofNat 64 2) .nil --checking edge cases
+def lh4 : HVector TyDenote.toType [RISCV64.Ty.bv ,RISCV64.Ty.bv] :=  HVector.cons (BitVec.ofNat 64 2) <| HVector.cons (BitVec.ofNat 64 2) .nil --checking edge cases
 def test_sllw : BitVec 64 := RISCVEg4.denote  (Ctxt.Valuation.ofHVector lh4)
 #eval test_sllw
 
@@ -70,7 +72,7 @@ def RISCVEg5 := [RV64_com| {
     %2 = "RV64.srlw" (%0, %1) : (!i64, !i64) -> (!i64)
     "return" (%2) : (!i64, !i64 ) -> ()
 }]
-def lh5 : HVector TyDenote.toType [toRISCV.Ty.bv ,toRISCV.Ty.bv] :=  HVector.cons (BitVec.ofNat 64 32) <| HVector.cons (BitVec.ofNat 64 1) .nil --checking edge cases
+def lh5 : HVector TyDenote.toType [RISCV64.Ty.bv ,RISCV64.Ty.bv] :=  HVector.cons (BitVec.ofNat 64 32) <| HVector.cons (BitVec.ofNat 64 1) .nil --checking edge cases
 def test_srlw : BitVec 64 := RISCVEg5.denote  (Ctxt.Valuation.ofHVector lh5)
 #eval test_srlw
 
@@ -80,7 +82,7 @@ def RISCVEg6 := [RV64_com| {
     %2 = "RV64.sraw" (%0, %1) : (!i64, !i64) -> (!i64)
     "return" (%2) : (!i64, !i64 ) -> ()
 }]
-def lh6 : HVector TyDenote.toType [toRISCV.Ty.bv ,toRISCV.Ty.bv] :=  HVector.cons (BitVec.ofNat 64 (16)) <| HVector.cons (BitVec.ofNat 64 2) .nil --checking edge cases
+def lh6 : HVector TyDenote.toType [RISCV64.Ty.bv ,RISCV64.Ty.bv] :=  HVector.cons (BitVec.ofNat 64 (16)) <| HVector.cons (BitVec.ofNat 64 2) .nil --checking edge cases
 def test_sraw : BitVec 64 := RISCVEg6.denote  (Ctxt.Valuation.ofHVector lh6)
 #eval test_sraw
 
@@ -92,7 +94,7 @@ def RISCVEg7 := [RV64_com| {
     "return" (%2) : (!i64, !i64 ) -> ()
 }]
 
-def lh7 : HVector TyDenote.toType [toRISCV.Ty.bv ,toRISCV.Ty.bv] :=  HVector.cons (BitVec.ofNat 64 1) <| HVector.cons (BitVec.ofNat 64 19) .nil
+def lh7 : HVector TyDenote.toType [RISCV64.Ty.bv ,RISCV64.Ty.bv] :=  HVector.cons (BitVec.ofNat 64 1) <| HVector.cons (BitVec.ofNat 64 19) .nil
 def test_add : BitVec 64 := RISCVEg7.denote  (Ctxt.Valuation.ofHVector lh7)
 #eval test_add
 
@@ -105,7 +107,7 @@ def RISCVEg8 := [RV64_com| {
 }]
 
 --testing the sign behavior edge cases , but this test should be true in the unisgned case
-def lh8 : HVector TyDenote.toType [toRISCV.Ty.bv ,toRISCV.Ty.bv] :=  HVector.cons (BitVec.ofNat 64 0) <| HVector.cons (BitVec.ofNat 64 (1)) .nil--checking edge cases
+def lh8 : HVector TyDenote.toType [RISCV64.Ty.bv ,RISCV64.Ty.bv] :=  HVector.cons (BitVec.ofNat 64 0) <| HVector.cons (BitVec.ofNat 64 (1)) .nil--checking edge cases
 def test_slt : BitVec 64 := RISCVEg8.denote  (Ctxt.Valuation.ofHVector lh8)
 #eval test_slt
 
@@ -115,7 +117,7 @@ def RISCVEg9 := [RV64_com| {
     %2 = "RV64.sltu" (%0, %1) : (!i64, !i64) -> (!i64)
     "return" (%2) : (!i64, !i64 ) -> ()
 }]
-def lh9 : HVector TyDenote.toType [toRISCV.Ty.bv ,toRISCV.Ty.bv] :=  HVector.cons (BitVec.ofNat 64 9223372036854775808) <| HVector.cons (BitVec.ofNat 64 (18446744073709551615)) .nil --18444 <= 92-- yields tue
+def lh9 : HVector TyDenote.toType [RISCV64.Ty.bv ,RISCV64.Ty.bv] :=  HVector.cons (BitVec.ofNat 64 9223372036854775808) <| HVector.cons (BitVec.ofNat 64 (18446744073709551615)) .nil --18444 <= 92-- yields tue
 --def lh9 : HVector TyDenote.toType [toRISCV.Ty.bv ,toRISCV.Ty.bv] :=  HVector.cons (BitVec.ofNat 64 10) <| HVector.cons (BitVec.ofNat 64 12) .nil --checking edge cases
 def test_sltu : BitVec 64 := RISCVEg9.denote  (Ctxt.Valuation.ofHVector lh9)
 #eval test_sltu
@@ -128,7 +130,7 @@ def RISCVEg10 := [RV64_com| {
 }]
 
 --bitwise and
-def lh10 : HVector TyDenote.toType [toRISCV.Ty.bv ,toRISCV.Ty.bv] :=  HVector.cons (BitVec.ofNat 64 7) <| HVector.cons (BitVec.ofNat 64 (7)) .nil --18444 <= 92-- yields tue
+def lh10 : HVector TyDenote.toType [RISCV64.Ty.bv ,RISCV64.Ty.bv] :=  HVector.cons (BitVec.ofNat 64 7) <| HVector.cons (BitVec.ofNat 64 (7)) .nil --18444 <= 92-- yields tue
 --def lh9 : HVector TyDenote.toType [toRISCV.Ty.bv ,toRISCV.Ty.bv] :=  HVector.cons (BitVec.ofNat 64 10) <| HVector.cons (BitVec.ofNat 64 12) .nil --checking edge cases
 def test_and : BitVec 64 := RISCVEg10.denote  (Ctxt.Valuation.ofHVector lh10)
 #eval test_and
@@ -140,7 +142,7 @@ def RISCVEg11 := [RV64_com| {
     %2 = "RV64.or" (%0, %1) : (!i64, !i64) -> (!i64)
     "return" (%2) : (!i64, !i64 ) -> ()
 }]
-def lh11 : HVector TyDenote.toType [toRISCV.Ty.bv ,toRISCV.Ty.bv] :=  HVector.cons (BitVec.ofNat 64 1) <| HVector.cons (BitVec.ofNat 64 (2)) .nil --18444 <= 92-- yields tue
+def lh11 : HVector TyDenote.toType [RISCV64.Ty.bv ,RISCV64.Ty.bv] :=  HVector.cons (BitVec.ofNat 64 1) <| HVector.cons (BitVec.ofNat 64 (2)) .nil --18444 <= 92-- yields tue
 --def lh9 : HVector TyDenote.toType [toRISCV.Ty.bv ,toRISCV.Ty.bv] :=  HVector.cons (BitVec.ofNat 64 10) <| HVector.cons (BitVec.ofNat 64 12) .nil --checking edge cases
 def test_or : BitVec 64 := RISCVEg11.denote  (Ctxt.Valuation.ofHVector lh11)
 #eval test_or
@@ -152,7 +154,7 @@ def RISCVEg12 := [RV64_com| {
     %2 = "RV64.xor" (%0, %1) : (!i64, !i64) -> (!i64)
     "return" (%2) : (!i64, !i64 ) -> ()
 }]
-def lh12 : HVector TyDenote.toType [toRISCV.Ty.bv ,toRISCV.Ty.bv] :=  HVector.cons (BitVec.ofNat 64 1) <| HVector.cons (BitVec.ofNat 64 1) .nil
+def lh12 : HVector TyDenote.toType [RISCV64.Ty.bv ,RISCV64.Ty.bv] :=  HVector.cons (BitVec.ofNat 64 1) <| HVector.cons (BitVec.ofNat 64 1) .nil
 def test_xor : BitVec 64 := RISCVEg12.denote  (Ctxt.Valuation.ofHVector lh12)
 #eval test_xor
 
@@ -162,7 +164,7 @@ def RISCVEg13 := [RV64_com| {
     %2 = "RV64.sll" (%0, %1) : (!i64, !i64) -> (!i64)
     "return" (%2) : (!i64, !i64 ) -> ()
 }]
-def lh13 : HVector TyDenote.toType [toRISCV.Ty.bv ,toRISCV.Ty.bv] :=  HVector.cons (BitVec.ofNat 64 1) <| HVector.cons (BitVec.ofNat 64 1) .nil
+def lh13 : HVector TyDenote.toType [RISCV64.Ty.bv ,RISCV64.Ty.bv] :=  HVector.cons (BitVec.ofNat 64 1) <| HVector.cons (BitVec.ofNat 64 1) .nil
 def test_sll : BitVec 64 := RISCVEg13.denote  (Ctxt.Valuation.ofHVector lh13)
 #eval test_sll
 
@@ -172,7 +174,7 @@ def RISCVEg14 := [RV64_com| {
     %2 = "RV64.srl" (%0, %1) : (!i64, !i64) -> (!i64)
     "return" (%2) : (!i64, !i64 ) -> ()
 }]
-def lh14 : HVector TyDenote.toType [toRISCV.Ty.bv ,toRISCV.Ty.bv] :=  HVector.cons (BitVec.ofNat 64 1) <| HVector.cons (BitVec.ofNat 64 1) .nil
+def lh14 : HVector TyDenote.toType [RISCV64.Ty.bv ,RISCV64.Ty.bv] :=  HVector.cons (BitVec.ofNat 64 1) <| HVector.cons (BitVec.ofNat 64 1) .nil
 def test_srl : BitVec 64 := RISCVEg14.denote  (Ctxt.Valuation.ofHVector lh14)
 #eval test_srl
 
@@ -184,7 +186,7 @@ def RISCVEg15 := [RV64_com| {
     %2 = "RV64.sub"  (%0, %1) : (!i64, !i64) -> (!i64)
     "return" (%2) : (!i64, !i64 ) -> ()
 }]
-def lh15 : HVector TyDenote.toType [toRISCV.Ty.bv ,toRISCV.Ty.bv] :=  HVector.cons (BitVec.ofNat 64 10) <| HVector.cons (BitVec.ofNat 64 0) .nil
+def lh15 : HVector TyDenote.toType [RISCV64.Ty.bv ,RISCV64.Ty.bv] :=  HVector.cons (BitVec.ofNat 64 10) <| HVector.cons (BitVec.ofNat 64 0) .nil
 def test_sub : BitVec 64 := RISCVEg15.denote  (Ctxt.Valuation.ofHVector lh15)
 #eval test_sub --interprete it as signed or unsigned
 
@@ -194,7 +196,7 @@ def RISCVEg16 := [RV64_com| {
     %2 = "RV64.addiw" (%0) { imm = 19 : !i64 } : ( !i64) -> (!i64)
     "return" (%2) : ( !i64 ) -> ()
 }]
-def lh16 : HVector TyDenote.toType [toRISCV.Ty.bv] := .cons (BitVec.ofNat 64 1) .nil
+def lh16 : HVector TyDenote.toType [RISCV64.Ty.bv] := .cons (BitVec.ofNat 64 1) .nil
 def test_addiw : BitVec 64 := RISCVEg16.denote  (Ctxt.Valuation.ofHVector lh16)
 #eval test_addiw
 
@@ -205,7 +207,7 @@ def RISCVEg17 := [RV64_com| {
     %2 = "RV64.lui" (%0) { imm = 19 : !i64 } : ( !i64) -> (!i64)
     "return" (%2) : ( !i64 ) -> ()
 }]
-def lh17 : HVector TyDenote.toType [toRISCV.Ty.bv] := .cons (BitVec.ofNat 64 1) .nil
+def lh17 : HVector TyDenote.toType [RISCV64.Ty.bv] := .cons (BitVec.ofNat 64 1) .nil
 def test_lui : BitVec 64 := RISCVEg17.denote  (Ctxt.Valuation.ofHVector lh17)
 #eval test_lui
 
@@ -215,7 +217,7 @@ def RISCVEg18 := [RV64_com| {
     %2 = "RV64.auipc" (%0) { imm = 19 : !i64 } : ( !i64) -> (!i64)
     "return" (%2) : ( !i64 ) -> ()
 }]
-def lh18 : HVector TyDenote.toType [toRISCV.Ty.bv] := .cons (BitVec.ofNat 64 1) .nil
+def lh18 : HVector TyDenote.toType [RISCV64.Ty.bv] := .cons (BitVec.ofNat 64 1) .nil
 def test_auipc : BitVec 64 := RISCVEg18.denote  (Ctxt.Valuation.ofHVector lh18)
 #eval test_auipc
 
@@ -225,7 +227,7 @@ def RISCVEg19 := [RV64_com| {
     %2 = "RV64.slliw" (%0) { shamt = 19 : !i64 } : ( !i64) -> (!i64)
     "return" (%2) : ( !i64 ) -> ()
 }]
-def lh19 : HVector TyDenote.toType [toRISCV.Ty.bv] := .cons (BitVec.ofNat 64 1) .nil
+def lh19 : HVector TyDenote.toType [RISCV64.Ty.bv] := .cons (BitVec.ofNat 64 1) .nil
 def test_slliw : BitVec 64 := RISCVEg19.denote  (Ctxt.Valuation.ofHVector lh18)
 #eval test_slliw
 
@@ -234,7 +236,7 @@ def RISCVEg20 := [RV64_com| {
     %2 = "RV64.srliw" (%0) { shamt = 19 : !i64 } : ( !i64) -> (!i64)
     "return" (%2) : ( !i64 ) -> ()
 }]
-def lh20 : HVector TyDenote.toType [toRISCV.Ty.bv] := .cons (BitVec.ofNat 64 1) .nil
+def lh20 : HVector TyDenote.toType [RISCV64.Ty.bv] := .cons (BitVec.ofNat 64 1) .nil
 def test_srliw : BitVec 64 := RISCVEg20.denote  (Ctxt.Valuation.ofHVector lh20)
 #eval test_srliw
 
@@ -243,7 +245,7 @@ def RISCVEg21 := [RV64_com| {
     %2 = "RV64.sraiw" (%0) { shamt = 19 : !i64 } : ( !i64) -> (!i64)
     "return" (%2) : ( !i64 ) -> ()
 }]
-def lh21 : HVector TyDenote.toType [toRISCV.Ty.bv] := .cons (BitVec.ofNat 64 1) .nil
+def lh21 : HVector TyDenote.toType [RISCV64.Ty.bv] := .cons (BitVec.ofNat 64 1) .nil
 def test_sraiw : BitVec 64 := RISCVEg21.denote  (Ctxt.Valuation.ofHVector lh21)
 #eval test_sraiw
 
@@ -253,7 +255,7 @@ def RISCVEg22 := [RV64_com| {
     %2 = "RV64.slli" (%0) { shamt = 19 : !i64 } : ( !i64) -> (!i64)
     "return" (%2) : ( !i64 ) -> ()
 }]
-def lh22 : HVector TyDenote.toType [toRISCV.Ty.bv] := .cons (BitVec.ofNat 64 1) .nil
+def lh22 : HVector TyDenote.toType [RISCV64.Ty.bv] := .cons (BitVec.ofNat 64 1) .nil
 def test_slli : BitVec 64 := RISCVEg22.denote  (Ctxt.Valuation.ofHVector lh22)
 #eval test_slli
 
@@ -263,7 +265,7 @@ def RISCVEg23 := [RV64_com| {
     %2 = "RV64.srli" (%0) { shamt = 0 : !i64 } : ( !i64) -> (!i64)
     "return" (%2) : ( !i64 ) -> ()
 }]
-def lh23 : HVector TyDenote.toType [toRISCV.Ty.bv] := .cons (BitVec.ofNat 64 1) .nil
+def lh23 : HVector TyDenote.toType [RISCV64.Ty.bv] := .cons (BitVec.ofNat 64 1) .nil
 def test_srli : BitVec 64 := RISCVEg23.denote  (Ctxt.Valuation.ofHVector lh23)
 #eval test_srli
 
@@ -273,7 +275,7 @@ def RISCVEg24 := [RV64_com| {
     %2 = "RV64.rem" (%0, %1) : ( !i64, !i64 ) -> (!i64)
     "return" (%2) : ( !i64, !i64 ) -> ()
 }]
-def lh24 : HVector TyDenote.toType [toRISCV.Ty.bv, toRISCV.Ty.bv] := HVector.cons (BitVec.ofNat 64 9) <| HVector.cons (BitVec.ofNat 64 (8)) .nil
+def lh24 : HVector TyDenote.toType [RISCV64.Ty.bv, RISCV64.Ty.bv] := HVector.cons (BitVec.ofNat 64 9) <| HVector.cons (BitVec.ofNat 64 (8)) .nil
 def test_rem : BitVec 64 := RISCVEg24.denote  (Ctxt.Valuation.ofHVector lh24)
 #eval test_rem
 
@@ -284,7 +286,7 @@ def RISCVEg25 := [RV64_com| {
     %2 = "RV64.mul" (%0, %1) : ( !i64, !i64 ) -> (!i64)
     "return" (%2) : ( !i64, !i64 ) -> ()
 }]
-def lh25 : HVector TyDenote.toType [toRISCV.Ty.bv, toRISCV.Ty.bv] := HVector.cons (BitVec.ofNat 64 7) <| HVector.cons (BitVec.ofNat 64 8) .nil
+def lh25 : HVector TyDenote.toType [RISCV64.Ty.bv, RISCV64.Ty.bv] := HVector.cons (BitVec.ofNat 64 7) <| HVector.cons (BitVec.ofNat 64 8) .nil
 def test_mul : BitVec 64 := RISCVEg25.denote  (Ctxt.Valuation.ofHVector lh25)
 #eval test_mul
 
@@ -294,7 +296,7 @@ def RISCVEg26 := [RV64_com| {
     %2 = "RV64.mulw" (%0, %1)  : ( !i64, !i64 ) -> (!i64)
     "return" (%2) : ( !i64, !i64 ) -> ()
 }]
-def lh26 : HVector TyDenote.toType [toRISCV.Ty.bv, toRISCV.Ty.bv] := HVector.cons (BitVec.ofNat 64 7) <| HVector.cons (BitVec.ofNat 64 8) .nil
+def lh26 : HVector TyDenote.toType [RISCV64.Ty.bv, RISCV64.Ty.bv] := HVector.cons (BitVec.ofNat 64 7) <| HVector.cons (BitVec.ofNat 64 8) .nil
 def test_mulw : BitVec 64 := RISCVEg26.denote  (Ctxt.Valuation.ofHVector lh26)
 #eval test_mulw
 
@@ -304,7 +306,7 @@ def RISCVEg27 := [RV64_com| {
     %2 = "RV64.div" (%0, %1) : ( !i64, !i64 ) -> (!i64)
     "return" (%2) : ( !i64, !i64 ) -> ()
 }]
-def lh27 : HVector TyDenote.toType [toRISCV.Ty.bv, toRISCV.Ty.bv] := HVector.cons (BitVec.ofNat 64 8) <| HVector.cons (BitVec.ofNat 64 4) .nil
+def lh27 : HVector TyDenote.toType [RISCV64.Ty.bv, RISCV64.Ty.bv] := HVector.cons (BitVec.ofNat 64 8) <| HVector.cons (BitVec.ofNat 64 4) .nil
 def test_div : BitVec 64 := RISCVEg27.denote  (Ctxt.Valuation.ofHVector lh27)
 #eval test_div
 
@@ -314,7 +316,7 @@ def RISCVEg28 := [RV64_com| {
     %2 = "RV64.divw" (%0, %1)  : ( !i64, !i64 ) -> (!i64)
     "return" (%2) : ( !i64, !i64 ) -> ()
 }]
-def lh28 : HVector TyDenote.toType [toRISCV.Ty.bv, toRISCV.Ty.bv] := HVector.cons (BitVec.ofNat 64 56) <| HVector.cons (BitVec.ofNat 64 8) .nil
+def lh28 : HVector TyDenote.toType [RISCV64.Ty.bv, RISCV64.Ty.bv] := HVector.cons (BitVec.ofNat 64 56) <| HVector.cons (BitVec.ofNat 64 8) .nil
 def test_divw : BitVec 64 := RISCVEg28.denote  (Ctxt.Valuation.ofHVector lh28)
 #eval test_divw
 
@@ -324,7 +326,7 @@ def RISCVEg29 := [RV64_com| {
     %2 = "RV64.addi" (%0)  { imm = 10 : !i64 } : ( !i64 ) -> (!i64)
     "return" (%2) : ( !i64 ) -> ()
 }]
-def lh29 : HVector TyDenote.toType [toRISCV.Ty.bv] := .cons (BitVec.ofNat 64 8) .nil
+def lh29 : HVector TyDenote.toType [RISCV64.Ty.bv] := .cons (BitVec.ofNat 64 8) .nil
 def test_addi : BitVec 64 := RISCVEg29.denote  (Ctxt.Valuation.ofHVector lh29)
 #eval test_addi
 
@@ -334,7 +336,7 @@ def RISCVEg30 := [RV64_com| {
     %2 = "RV64.slti" (%0)  { imm = 10 : !i64 } : ( !i64 ) -> (!i64)
     "return" (%2) : ( !i64 ) -> ()
 }]
-def lh30 : HVector TyDenote.toType [toRISCV.Ty.bv] := .cons (BitVec.ofNat 64 1) .nil
+def lh30 : HVector TyDenote.toType [RISCV64.Ty.bv] := .cons (BitVec.ofNat 64 1) .nil
 def test_slti : BitVec 64 := RISCVEg30.denote  (Ctxt.Valuation.ofHVector lh30)
 #eval test_slti
 
@@ -344,7 +346,7 @@ def RISCVEg31 := [RV64_com| {
     %2 = "RV64.sltiu" (%0)  { imm = 10 : !i64 } : ( !i64 ) -> (!i64)
     "return" (%2) : ( !i64 ) -> ()
 }]
-def lh31 : HVector TyDenote.toType [toRISCV.Ty.bv] := .cons (BitVec.ofNat 64 8) .nil
+def lh31 : HVector TyDenote.toType [RISCV64.Ty.bv] := .cons (BitVec.ofNat 64 8) .nil
 def test_sltiu : BitVec 64 := RISCVEg31.denote  (Ctxt.Valuation.ofHVector lh31)
 #eval test_sltiu
 
@@ -354,7 +356,7 @@ def RISCVEg32 := [RV64_com| {
     %2 = "RV64.andi" (%0)  { imm = 15 : !i64 } : ( !i64 ) -> (!i64)
     "return" (%2) : ( !i64 ) -> ()
 }]
-def lh32 : HVector TyDenote.toType [toRISCV.Ty.bv] := .cons (BitVec.ofNat 64 16) .nil
+def lh32 : HVector TyDenote.toType [RISCV64.Ty.bv] := .cons (BitVec.ofNat 64 16) .nil
 def test_andi : BitVec 64 := RISCVEg32.denote  (Ctxt.Valuation.ofHVector lh32)
 #eval test_andi
 
@@ -364,7 +366,7 @@ def RISCVEg33 := [RV64_com| {
     %2 = "RV64.ori" (%0)  { imm = 10 : !i64 } : ( !i64 ) -> (!i64)
     "return" (%2) : ( !i64 ) -> ()
 }]
-def lh33 : HVector TyDenote.toType [toRISCV.Ty.bv] := .cons (BitVec.ofNat 64 8) .nil
+def lh33 : HVector TyDenote.toType [RISCV64.Ty.bv] := .cons (BitVec.ofNat 64 8) .nil
 def test_ori : BitVec 64 := RISCVEg33.denote  (Ctxt.Valuation.ofHVector lh33)
 #eval test_ori
 
@@ -374,7 +376,7 @@ def RISCVEg34 := [RV64_com| {
     %2 = "RV64.xori" (%0)  { imm = 7 : !i64 } : ( !i64 ) -> (!i64)
     "return" (%2) : ( !i64 ) -> ()
 }]
-def lh34 : HVector TyDenote.toType [toRISCV.Ty.bv] := .cons (BitVec.ofNat 64 2) .nil
+def lh34 : HVector TyDenote.toType [RISCV64.Ty.bv] := .cons (BitVec.ofNat 64 2) .nil
 def test_xori : BitVec 64 := RISCVEg34.denote  (Ctxt.Valuation.ofHVector lh34)
 #eval test_xori
 
@@ -384,7 +386,7 @@ def RISCVEg35 := [RV64_com| {
     %2 = "RV64.czero.eqz" (%0, %1) : (!i64, !i64) -> (!i64)
     "return" (%2) : (!i64, !i64 ) -> ()
 }]
-def lh35 : HVector TyDenote.toType [toRISCV.Ty.bv ,toRISCV.Ty.bv] :=  HVector.cons (BitVec.ofNat 64 1) <| HVector.cons (BitVec.ofNat 64 1) .nil
+def lh35 : HVector TyDenote.toType [RISCV64.Ty.bv ,RISCV64.Ty.bv] :=  HVector.cons (BitVec.ofNat 64 1) <| HVector.cons (BitVec.ofNat 64 1) .nil
 def test_czero.eqz : BitVec 64 := RISCVEg35.denote  (Ctxt.Valuation.ofHVector lh35)
 #eval test_czero.eqz --interprete it as signed or unsigned
 
@@ -394,7 +396,7 @@ def RISCVEg36 := [RV64_com| {
     %2 = "RV64.czero.nez" (%0, %1) : (!i64, !i64) -> (!i64)
     "return" (%2) : (!i64, !i64 ) -> ()
 }]
-def lh36 : HVector TyDenote.toType [toRISCV.Ty.bv ,toRISCV.Ty.bv] :=  HVector.cons (BitVec.ofNat 64 19) <| HVector.cons (BitVec.ofNat 64 0) .nil
+def lh36 : HVector TyDenote.toType [RISCV64.Ty.bv ,RISCV64.Ty.bv] :=  HVector.cons (BitVec.ofNat 64 19) <| HVector.cons (BitVec.ofNat 64 0) .nil
 def test_czero.nez : BitVec 64 := RISCVEg36.denote  (Ctxt.Valuation.ofHVector lh36)
 #eval test_czero.nez --interprete it as signed or unsigned
 
@@ -404,7 +406,7 @@ def RISCVEg37 := [RV64_com| {
     %2 = "RV64.sext.b" (%0) : ( !i64) -> (!i64)
     "return" (%2) : (!i64 ) -> ()
 }]
-def lh37 : HVector TyDenote.toType [toRISCV.Ty.bv] :=  HVector.cons (BitVec.ofNat 64 0) .nil
+def lh37 : HVector TyDenote.toType [RISCV64.Ty.bv] :=  HVector.cons (BitVec.ofNat 64 0) .nil
 def test_sext.b : BitVec 64 := RISCVEg37.denote  (Ctxt.Valuation.ofHVector lh37)
 #eval test_sext.b
 
@@ -414,7 +416,7 @@ def RISCVEg38 := [RV64_com| {
     %2 = "RV64.sext.h" (%0) : ( !i64) -> (!i64)
     "return" (%2) : (!i64 ) -> ()
 }]
-def lh38 : HVector TyDenote.toType [toRISCV.Ty.bv] :=  HVector.cons (BitVec.ofNat 64 (1)) .nil
+def lh38 : HVector TyDenote.toType [RISCV64.Ty.bv] :=  HVector.cons (BitVec.ofNat 64 (1)) .nil
 def test_sext.h : BitVec 64 := RISCVEg38.denote  (Ctxt.Valuation.ofHVector lh38)
 #eval test_sext.h
 
@@ -424,7 +426,7 @@ def RISCVEg39 := [RV64_com| {
     %2 = "RV64.zext.h" (%0) : ( !i64) -> (!i64)
     "return" (%2) : (!i64 ) -> ()
 }]
-def lh39 : HVector TyDenote.toType [toRISCV.Ty.bv] :=  HVector.cons (BitVec.ofNat 64 5) .nil
+def lh39 : HVector TyDenote.toType [RISCV64.Ty.bv] :=  HVector.cons (BitVec.ofNat 64 5) .nil
 def test_zext.h : BitVec 64 := RISCVEg39.denote  (Ctxt.Valuation.ofHVector lh39)
 #eval test_zext.h
 
@@ -434,7 +436,7 @@ def RISCVEg40 := [RV64_com| {
     %2 = "RV64.bclr" (%0, %1) : ( !i64,!i64 ) -> (!i64)
     "return" (%2) : (!i64, !i64 ) -> ()
 }]
-def lh40 : HVector TyDenote.toType [toRISCV.Ty.bv, toRISCV.Ty.bv ] := HVector.cons (BitVec.ofNat 64 8) <| HVector.cons (BitVec.ofNat 64 3) .nil
+def lh40 : HVector TyDenote.toType [RISCV64.Ty.bv, RISCV64.Ty.bv ] := HVector.cons (BitVec.ofNat 64 8) <| HVector.cons (BitVec.ofNat 64 3) .nil
 def test_bclr: BitVec 64 := RISCVEg40.denote  (Ctxt.Valuation.ofHVector lh40)
 #eval test_bclr
 
@@ -444,7 +446,7 @@ def RISCVEg41 := [RV64_com| {
     %2 = "RV64.bext" (%0, %1) : ( !i64,!i64 ) -> (!i64)
     "return" (%2) : (!i64, !i64 ) -> ()
 }]
-def lh41 : HVector TyDenote.toType [toRISCV.Ty.bv, toRISCV.Ty.bv ] := HVector.cons (BitVec.ofNat 64 3) <| HVector.cons (BitVec.ofNat 64 2) .nil
+def lh41 : HVector TyDenote.toType [RISCV64.Ty.bv, RISCV64.Ty.bv] := HVector.cons (BitVec.ofNat 64 3) <| HVector.cons (BitVec.ofNat 64 2) .nil
 def test_bext: BitVec 64 := RISCVEg41.denote  (Ctxt.Valuation.ofHVector lh41)
 #eval test_bext
 
@@ -454,7 +456,7 @@ def RISCVEg42 := [RV64_com| {
     %2 = "RV64.binv" (%0, %1) : ( !i64, !i64 ) -> (!i64)
     "return" (%2) : (!i64, !i64 ) -> ()
 }]
-def lh42 : HVector TyDenote.toType [toRISCV.Ty.bv, toRISCV.Ty.bv ] := HVector.cons (BitVec.ofNat 64 0) <| HVector.cons (BitVec.ofNat 64 0) .nil
+def lh42 : HVector TyDenote.toType [RISCV64.Ty.bv, RISCV64.Ty.bv ] := HVector.cons (BitVec.ofNat 64 0) <| HVector.cons (BitVec.ofNat 64 0) .nil
 def test_inv: BitVec 64 := RISCVEg42.denote  (Ctxt.Valuation.ofHVector lh42)
 #eval test_inv
 
@@ -464,7 +466,7 @@ def RISCVEg43 := [RV64_com| {
     %2 = "RV64.bset" (%0, %1) : ( !i64, !i64 ) -> (!i64)
     "return" (%2) : (!i64, !i64 ) -> ()
 }]
-def lh43 : HVector TyDenote.toType [toRISCV.Ty.bv, toRISCV.Ty.bv ] := HVector.cons (BitVec.ofNat 64 1) <| HVector.cons (BitVec.ofNat 64 0) .nil
+def lh43 : HVector TyDenote.toType [RISCV64.Ty.bv, RISCV64.Ty.bv ] := HVector.cons (BitVec.ofNat 64 1) <| HVector.cons (BitVec.ofNat 64 0) .nil
 def test_bset: BitVec 64 := RISCVEg43.denote  (Ctxt.Valuation.ofHVector lh43)
 #eval test_bset
 
@@ -474,7 +476,7 @@ def RISCVEg44 := [RV64_com| {
     %2 = "RV64.rolw" (%0, %1) : ( !i64, !i64 ) -> (!i64)
     "return" (%2) : (!i64, !i64 ) -> ()
 }]
-def lh44 : HVector TyDenote.toType [toRISCV.Ty.bv, toRISCV.Ty.bv ] := HVector.cons (BitVec.ofNat 64 64) <| HVector.cons (BitVec.ofNat 64 4) .nil
+def lh44 : HVector TyDenote.toType [RISCV64.Ty.bv, RISCV64.Ty.bv] := HVector.cons (BitVec.ofNat 64 64) <| HVector.cons (BitVec.ofNat 64 4) .nil
 def test_rolw: BitVec 64 := RISCVEg44.denote  (Ctxt.Valuation.ofHVector lh44)
 #eval test_rolw
 
@@ -484,7 +486,7 @@ def RISCVEg45 := [RV64_com| {
     %2 = "RV64.rorw" (%0, %1) : ( !i64, !i64 ) -> (!i64)
     "return" (%2) : (!i64, !i64 ) -> ()
 }]
-def lh45 : HVector TyDenote.toType [toRISCV.Ty.bv, toRISCV.Ty.bv ] := HVector.cons (BitVec.ofNat 64 64) <| HVector.cons (BitVec.ofNat 64 4) .nil
+def lh45 : HVector TyDenote.toType [RISCV64.Ty.bv, RISCV64.Ty.bv] := HVector.cons (BitVec.ofNat 64 64) <| HVector.cons (BitVec.ofNat 64 4) .nil
 def test_rorw: BitVec 64 := RISCVEg45.denote  (Ctxt.Valuation.ofHVector lh45)
 #eval test_rorw
 
@@ -494,7 +496,7 @@ def RISCVEg46 := [RV64_com| {
     %2 = "RV64.bclri" (%0) { imm = 1 : !i64 } : ( !i64) -> (!i64)
     "return" (%2) : ( !i64 ) -> ()
 }]
-def lh46 : HVector TyDenote.toType [toRISCV.Ty.bv] := .cons (BitVec.ofNat 64 7) .nil
+def lh46 : HVector TyDenote.toType [RISCV64.Ty.bv] := .cons (BitVec.ofNat 64 7) .nil
 def test_bclri : BitVec 64 := RISCVEg46.denote  (Ctxt.Valuation.ofHVector lh46)
 #eval test_bclri
 
@@ -504,7 +506,7 @@ def RISCVEg47 := [RV64_com| {
     %2 = "RV64.bexti" (%0) { imm = 63 : !i64 } : ( !i64) -> (!i64)
     "return" (%2) : ( !i64 ) -> ()
 }]
-def lh47 : HVector TyDenote.toType [toRISCV.Ty.bv] := .cons (BitVec.ofNat 64 7) .nil
+def lh47 : HVector TyDenote.toType [RISCV64.Ty.bv] := .cons (BitVec.ofNat 64 7) .nil
 def test_bexit : BitVec 64 := RISCVEg47.denote  (Ctxt.Valuation.ofHVector lh47)
 #eval test_bexit
 
@@ -514,7 +516,7 @@ def RISCVEg48 := [RV64_com| {
     %2 = "RV64.binvi" (%0) { imm = 2 : !i64 } : ( !i64) -> (!i64)
     "return" (%2) : ( !i64 ) -> ()
 }]
-def lh48 : HVector TyDenote.toType [toRISCV.Ty.bv] := .cons (BitVec.ofNat 64 0) .nil
+def lh48 : HVector TyDenote.toType [RISCV64.Ty.bv] := .cons (BitVec.ofNat 64 0) .nil
 def test_binvi : BitVec 64 := RISCVEg48.denote  (Ctxt.Valuation.ofHVector lh48)
 #eval test_binvi
 
@@ -524,7 +526,7 @@ def RISCVEg49 := [RV64_com| {
     %2 = "RV64.bseti" (%0) { imm = 63 : !i64 } : ( !i64) -> (!i64)
     "return" (%2) : ( !i64 ) -> ()
 }]
-def lh49 : HVector TyDenote.toType [toRISCV.Ty.bv] := .cons (BitVec.ofNat 64 0) .nil
+def lh49 : HVector TyDenote.toType [RISCV64.Ty.bv] := .cons (BitVec.ofNat 64 0) .nil
 def test_seti : BitVec 64 := RISCVEg49.denote  (Ctxt.Valuation.ofHVector lh49)
 #eval test_seti
 
@@ -534,7 +536,7 @@ def RISCVEg50 := [RV64_com| {
     %2 = "RV64.const" () { val = 250 : !i64 } : ( !i64) -> (!i64)
     "return" (%2) : ( !i64 ) -> ()
 }]
-def lh50 : HVector TyDenote.toType [toRISCV.Ty.bv] := .cons (BitVec.ofNat 64 1) .nil
+def lh50 : HVector TyDenote.toType [RISCV64.Ty.bv] := .cons (BitVec.ofNat 64 1) .nil
 def test_const : BitVec 64 := RISCVEg50.denote  (Ctxt.Valuation.ofHVector lh50)
 #eval test_const
 
@@ -547,7 +549,7 @@ def RISCVEg200 := [RV64_com| {
     "return" (%5) : ( !i64 ) -> ()
 }]
 
-def lh200 : HVector TyDenote.toType [toRISCV.Ty.bv,toRISCV.Ty.bv ] := HVector.cons (BitVec.ofNat 64 1) <| HVector.cons (BitVec.ofNat 64 3) .nil
+def lh200 : HVector TyDenote.toType [RISCV64.Ty.bv,RISCV64.Ty.bv] := HVector.cons (BitVec.ofNat 64 1) <| HVector.cons (BitVec.ofNat 64 3) .nil
 def test_RISCVEg200 : BitVec 64 := RISCVEg200.denote  (Ctxt.Valuation.ofHVector lh200)
 #eval test_RISCVEg200
 
@@ -558,7 +560,7 @@ def RISCVEg51 := [RV64_com| {
     %2 = "RV64.srai" (%0) { shamt = 1 : !i64 } : ( !i64) -> (!i64)
     "return" (%2) : ( !i64 ) -> ()
 }]
-def lh51 : HVector TyDenote.toType [toRISCV.Ty.bv] := .cons (BitVec.ofNat 64 16) .nil
+def lh51 : HVector TyDenote.toType [RISCV64.Ty.bv] := .cons (BitVec.ofNat 64 16) .nil
 def test_srai : BitVec 64 := RISCVEg51.denote  (Ctxt.Valuation.ofHVector lh51)
 #eval test_srai
 
@@ -568,7 +570,7 @@ def RISCVEg52 := [RV64_com| {
     %2 = "RV64.sra" (%0, %1 ) : (!i64,!i64) -> (!i64)
     "return" (%2) : ( !i64 ) -> ()
 }]
-def lh52 : HVector TyDenote.toType [toRISCV.Ty.bv, toRISCV.Ty.bv ] := HVector.cons (BitVec.ofNat 64 16) <| HVector.cons (BitVec.ofNat 64 2) .nil
+def lh52 : HVector TyDenote.toType [RISCV64.Ty.bv, RISCV64.Ty.bv] := HVector.cons (BitVec.ofNat 64 16) <| HVector.cons (BitVec.ofNat 64 2) .nil
 def test_sra : BitVec 64 := RISCVEg52.denote (Ctxt.Valuation.ofHVector lh52)
 #eval test_sra
 
@@ -577,7 +579,7 @@ def RISCVEg53 := [RV64_com| {
     %2 = "RV64.rol" (%0, %1 ) : (!i64,!i64) -> (!i64)
     "return" (%2) : ( !i64 ) -> ()
 }]
-def lh53 : HVector TyDenote.toType [toRISCV.Ty.bv, toRISCV.Ty.bv ]
+def lh53 : HVector TyDenote.toType [RISCV64.Ty.bv, RISCV64.Ty.bv]
   := HVector.cons (BitVec.ofNat 64 2) <| HVector.cons (BitVec.ofNat 64 1) .nil
 
 def test_rol : BitVec 64 := RISCVEg53.denote (Ctxt.Valuation.ofHVector lh53)
@@ -589,7 +591,7 @@ def RISCVEg54 := [RV64_com| {
     %2 = "RV64.ror" (%0, %1 ) : (!i64,!i64) -> (!i64)
     "return" (%2) : ( !i64 ) -> ()
 }]
-def lh54 : HVector TyDenote.toType [toRISCV.Ty.bv, toRISCV.Ty.bv ]
+def lh54 : HVector TyDenote.toType [RISCV64.Ty.bv, RISCV64.Ty.bv]
   := HVector.cons (BitVec.ofNat 64 8) <| HVector.cons (BitVec.ofNat 64 1) .nil
 
 def test_ror : BitVec 64 := RISCVEg54.denote (Ctxt.Valuation.ofHVector lh54)
@@ -601,7 +603,7 @@ def RISCVEg55 := [RV64_com| {
     %2 = "RV64.const" () { val = 670 : !i64 } : ( !i64) -> (!i64)
     "return" (%2) : ( !i64 ) -> ()
 }]
-def lh55 : HVector TyDenote.toType ([] : List toRISCV.Ty) := .nil
+def lh55 : HVector TyDenote.toType ([] : List RISCV64.Ty) := .nil
 def test_const1 : BitVec 64 := RISCVEg55.denote  (Ctxt.Valuation.ofHVector lh55)
 #eval test_const1
 #check TyDenote.toType
