RiscvDialect/RISCV64/all.lean
@@ -1,0 +1,3 @@
+import RiscvDialect.RISCV64.Syntax
+import RiscvDialect.RISCV64.Base
+import RiscvDialect.RISCV64.Semantics
